\begin{solution} 

Start with
    \begin{align*}
      u\left(y, z\right) = \sum_{n=1}^{\infty}{\beta_{n}\left(z\right)\sin\left(\frac{n\pi}{a}y\right)}.
    \end{align*}

Take second-order derivatives:
    \begin{align*}
      \partial_{y}^{2}u &= - \sum_{n=1}^{\infty} (\frac{n\pi}{a})^2 {\beta_{n} \left(z\right)\sin\left(\frac{n\pi}{a}y\right)} \\
      \partial_{z}^{2}u &= \sum_{n=1}^{\infty}{\beta_{n}^{\prime\prime} \left(z\right)\sin\left(\frac{n\pi}{a}y\right)}
    \end{align*}

Bring into the original PDE:
    \begin{align*}
      \partial_{y}^{2}u + \partial_{z}^{2}u = Q
    \end{align*}

Leads to:
      \begin{align*}
        \sum_{n=1}^{\infty}{\beta_{n}^{\prime\prime}\sin\left(\dfrac{n\pi}{a}y\right)} -
\sum_{n=1}^{\infty}{\beta_{n}\left(\dfrac{n\pi}{a}\right)^{2}\sin\left(\dfrac{n\pi}{a}y\right)} = Q
      \end{align*}

Multiply by $\sin\left(\dfrac{m\pi}{a}y\right)$ and integrate over $y$:
      \begin{align*}
        &\int_{0}^{a}{\sum_{n=1}^{\infty}{\beta_{n}^{\prime\prime}\sin\left(\dfrac{n\pi}{a}y\right)\sin\left(\dfrac{m\pi}{a}y\right)}
\ \mathrm{d}y} -
\int_{0}^{a}{\sum_{n=1}^{\infty}{\beta_{n}\left(\dfrac{n\pi}{a}\right)^{2}\sin\left(\dfrac{n\pi}{a}y\right)\sin\left(\dfrac{m\pi}{a}y\right)}
\ \mathrm{d}y} = \nonumber \\
        &\hspace{2.0em}\int_{0}^{a}{Q\sin\left(\dfrac{m\pi}{a}y\right) \ \mathrm{d}y}
      \end{align*}

Using the orthogonality of sines, it becomes:
        \begin{align*}
           \dfrac{a}{2}\beta_{m}^{\prime\prime} - \dfrac{a}{2}(\dfrac{m\pi}{a})^{2}\beta_{m} =\int_{0}^{a}{Q\sin\left(\dfrac{m\pi}{a}y\right) \ \mathrm{d}y}
        \end{align*}

Replace $m$ by $n$ (they are interchangeable at the above step) and use $\gamma_{n}=\dfrac{n\pi}{a}$, the above reduces to the desired result:
        \begin{align*}
          \beta_{n}^{\prime\prime} - \gamma_{n}^{2}\beta_{n} = \dfrac{2}{a}\int_{0}^{a}{Q\sin\left(\gamma_{n}y\right) \ \mathrm{d}y}
        \end{align*}

\end{solution} 