\begin{solution} 

The homogeneous ODE can be factored (in terms of operators) as:
    \begin{align*}
    (\dfrac{d}{dz}-\gamma_{n}) (\dfrac{d}{dz}+\gamma_{n})\beta_{n}= 0
    \end{align*}

The solution needs to satisfy either:
    \begin{align*}
    (\dfrac{d}{dz}-\gamma_{n})\beta_{n} = 0 \text{  or  } (\dfrac{d}{dz}+\gamma_{n})\beta_{n} = 0
    \end{align*}
    
The solution to each first-order ODE is:
    \begin{align*}
    \beta_{n} = e^{\gamma_{n}z} \text{  or  } \beta_{n} = e^{-\gamma_{n}z}
    \end{align*}

Any of their linear combinations are correct solutions:
    \begin{align*}
    \beta_{n}^{H} = k_1 e^{\gamma_{n}z} + k_2 e^{-\gamma_{n}z}
    \end{align*}

Or, equivalently
    \begin{align*}
      \beta_{n}^{H} = c_{1} \sinh\left(\gamma_{n}z\right) + c_{2} \cosh\left(\gamma_{n}z\right)
    \end{align*}

\end{solution} 