\begin{solution} 

Bring the complete form of $\beta_{n}\left(z\right)$ (obtained in the previous question) into the original expansion:

    \begin{align*}
      u\left(y, z\right) = \sum_{n=1}^{\infty}{\beta_{n}\left(z\right)\sin\left(\frac{n\pi}{a}y\right)}.
    \end{align*}

Leads to the desired result that

    \begin{align*}
      u\left(y,z\right) = \sum_{n=1}^{\infty}{2C_{n} 
        \sinh\left(\dfrac{\gamma_{n}}{2}\left(z-b\right)\right)\left[\cosh\left(\dfrac{\gamma_{n}}{2}\left(z+b\right)\right) - 
          \cosh\left(\dfrac{\gamma_{n}}{2}\left(z-b\right)\right)\right]\sin\left(\gamma_{n}y\right)}.
    \end{align*}
    
\begin{itemize}
\item The boundary condition $u(y=0) = u(y=a) = 0$ is satisfied as $\sin\left(\frac{n\pi}{a}y\right) = 0$ when $y=0$ or $y=a$
\item $u(z=b) = 0$ is satisfied as $\sinh\left(\dfrac{\gamma_{n}}{2}\left(z-b\right)\right)=0$ when $z=b$.

\item $u(z=b) = 0$ is satisfied as $[\cosh\left(\dfrac{\gamma_{n}}{2}\left(z+b\right)\right)-\cosh\left(\dfrac{\gamma_{n}}{2}\left(z-b\right)\right) = 0$ when $z=0$.
\end{itemize}

So all boundary conditions are satisfied.

\end{solution} 