\begin{solution}
Now, let 

$$w^h = \sum_{A=1}^{n}W_A N_A(x) \qquad N_A(1) = 0, \, \forall \, A=[1, ..., n]$$
$$u^h = \sum_{B=1}^{n}U_B N_B(x) + u_0 N_{n + 1}(x) \qquad N_B(0) = 0 , \, \forall \, B=[1, ..., n], \, N_{n+1}(0) = 0$$\\

Therefore, defining: 

$$v^h = \sum_{B=1}^{n}U_B N_B(x)$$

$$g^h = u_0 N_{n + 1}(x) $$

We proceed now to plug these values into the Galerkin Statement:

\begin{dmath}
a \int_0^{1} \Big(\sum_{A=1}^{n}W_A N_A(x)\Big) \partial_x \Big(\sum_{B=1}^{n}U_B N_B(x)\Big) dx - \lambda\int_0^{1} \Big(\sum_{A=1}^{n}W_A N_A(x)\Big) \Big(\sum_{B=1}^{n}U_B N_B(x)\Big) dx + k\int_0^1 \partial_x \Big(\sum_{A=1}^{n}W_A N_A(x)\Big) \partial_x \Big(\sum_{B=1}^{n}U_B N_B(x)\Big) dx= \int_0^1 f \Big(\sum_{A=1}^{n}W_A N_A(x)\Big) dx + b_1 \Big(\sum_{A=1}^{n}W_A N_A(1)\Big) - a \int_0^{1} \Big(\sum_{A=1}^{n}W_A N_A(x)\Big) \partial_x \Big(u_0 N_{n + 1}(x)\Big) dx + \lambda\int_0^{1} \Big(\sum_{A=1}^{n}W_A N_A(x)\Big) \Big(u_0 N_{n + 1}(x)\Big) dx - k\int_0^1 \partial_x \Big(\sum_{A=1}^{n}W_A N_A(x)\Big) \partial_x \Big(u_0 N_{n + 1}(x)\Big) dx
\end{dmath}

\begin{dmath}
\sum_{A=1}^{n}W_A \Bigg[ a \int_0^{1} N_A(x) \partial_x \Big(\sum_{B=1}^{n}U_B N_B(x)\Big) dx - \lambda\int_0^{1} N_A(x) \Big(\sum_{B=1}^{n}U_B N_B(x)\Big) dx + k\int_0^1 \partial_x N_A(x) \partial_x \Big(\sum_{B=1}^{n}U_B N_B(x)\Big) dx - \int_0^1 f N_A(x) dx - b_1 N_A(1) + a \int_0^{1} N_A(x) \partial_x \Big(u_0 N_{n + 1}(x)\Big) dx - \lambda\int_0^{1} N_A(x) \Big(u_0 N_{n + 1}(x)\Big) dx + k\int_0^1 \partial_x N_A(x) \partial_x \Big(u_0 N_{n + 1}(x)\Big) dx \Bigg] = 0
\end{dmath}
\end{solution}
\begin{solution}
\begin{dmath}
\sum_{A=1}^{n}W_A \Bigg[ \sum_{B=1}^{n}U_B \Bigg( a \int_0^{1} N_A(x) \partial_x N_B(x) dx - \lambda\int_0^{1} N_A(x) N_B(x) dx + k\int_0^1 \partial_x N_A(x) \partial_x N_B(x) dx \Bigg) - \int_0^1 f N_A(x) dx - b_1 N_A(1) + a \int_0^{1} N_A(x) \partial_x \Big(u_0 N_{n + 1}(x)\Big) dx - \lambda\int_0^{1} N_A(x) u_0 N_{n + 1}(x) dx + k\int_0^1 \partial_x N_A(x) \partial_x \Big(u_0 N_{n + 1}(x)\Big) dx \Bigg] = 0
\end{dmath}

To simplify the formula, let us redefine some of the expressions above:

\begin{align}
\kappa_{AB} &= a \int_0^{1} N_A(x) \partial_x N_B(x) dx - \lambda\int_0^{1} N_A(x) N_B(x) dx + k\int_0^1 \partial_x N_A(x) \partial_x N_B(x) dx \\
F_a &= \int_0^1 f N_A(x) dx\\
G_a &= a \int_0^{1} N_A(x) \partial_x \Big(u_0 N_{n + 1}(x)\Big) dx\\
H_a &= b_1 N_A(1)\\
I_a &= \lambda\int_0^{1} N_A(x) u_0 N_{n + 1}(x) dx\\
J_a &= k\int_0^1 \partial_x N_A(x) \partial_x \Big(u_0 N_{n + 1}(x)\Big) dx\\
\mathbf{F}_A &= F_a + G_a - H_a + I_a - J_a
\end{align}

Therefore, rewriting our expression above as:

\begin{dmath}
\sum_{A=1}^{n}W_A \Big[ \Big( \sum_{B=1}^{n}U_B( \kappa_{AB}) - \mathbf{F}_A\Big] = 0
\end{dmath}

In order for the expression to hold, the following must be true:\\

$$\sum_{B=1}^{n}U_B( \kappa_{AB}) = \mathbf{F}_A$$
\end{solution}